theories/Theorems/Order.v
@@ -1,4 +1,5 @@
 Require Import Utf8.Spec.
+From Coq Require Import Lists.List. Import ListNotations.
 
 Ltac crush_bits :=
   let B := fresh "B" in
@@ -20,20 +21,10 @@ Ltac to_bits byte :=
   in 
   match type of byte with
   | Spec.codepoint =>
-      unfold Spec.codepoint, Spec.b4 in byte;
+      unfold Spec.codepoint in byte;
       let b := fresh "b" in
       destruct byte as [[[[[b b4_1] b4_2] b4_3] b4_4] b4_5];
       break_bit b4_1; break_bit b4_2; break_bit b4_3; break_bit b4_4; break_bit b4_5
-  | Spec.b7 =>
-      unfold Spec.b7 in byte; break_bit byte
-  | Spec.b6 =>
-      unfold Spec.b6 in byte; break_bit byte
-  | Spec.b5 =>
-      unfold Spec.b5 in byte; break_bit byte
-  | Spec.b4 =>
-      unfold Spec.b4 in byte; break_bit byte
-  | Spec.b3 =>
-      unfold Spec.b3 in byte; break_bit byte
   | Byte.byte =>
       let B := fresh "B" in
       let eqn_name := fresh "byte_bits" in
@@ -44,240 +35,29 @@ Ltac to_bits byte :=
       rewrite Byte.of_bits_to_bits in eqn_name
   end.
 
-Definition antisymmetric {T} (comp: T -> T -> comparison) :=
-  forall t1 t2,
-    match comp t1 t2 with
-    | More => comp t2 t1 = Less
-    | Less => comp t2 t1 = More
-    | Equal => t1 = t2
-    end.
-
-Definition transitive {T} (comp: T -> T -> comparison) :=
-  forall t1 t2 t3,
-    comp t1 t2 = comp t2 t3 -> comp t1 t2 = comp t1 t3.
-
-Definition antisymmetric_reflexive {T} (comp: T -> T -> comparison):
-  antisymmetric comp ->
-  forall t, comp t t = Equal.
-Proof.
-  intros comp_spec t.
-  unfold antisymmetric in comp_spec.
-  specialize (comp_spec t t).
-  destruct (comp t t) eqn:comp_t; [discriminate | reflexivity | discriminate].
-Qed.
-
-Lemma if_equal_pair_antisymmetric {T} (comp: T -> T -> comparison) :
-    antisymmetric comp -> 
-    antisymmetric
-      (fun (a b: T * T) =>
-         let '(a1, a2) := a in
-         let '(b1, b2) := b in
-         if_equal (comp a1 b1) (comp a2 b2)).
-Proof.
-  intros comp_spec a b.
-  destruct a as [a1 a2]; destruct b as [b1 b2].
-  unfold if_equal. simpl.
-  specialize (comp_spec a1 b1) as comp_spec1.
-  destruct (comp a1 b1) eqn:comp1; rewrite comp_spec1; auto. subst. rewrite comp1.
-  specialize (comp_spec a2 b2) as comp_spec2.
-  destruct (comp a2 b2) eqn:comp2; subst; auto.
-Qed.
-
-Lemma if_equal_pair_transitive {T} (comp: T -> T -> comparison) :
-  antisymmetric comp ->
-  transitive comp -> 
-  transitive 
-      (fun (a b: T * T) =>
-         let '(a1, a2) := a in
-         let '(b1, b2) := b in
-         if_equal (comp a1 b1) (comp a2 b2)).
-Proof.
-  intros comp_anti comp_trans a b c comp_eq.
-  destruct a as [a1 a2]; destruct b as [b1 b2]. destruct c as [c1 c2].
-  unfold if_equal. simpl.
-  destruct (comp a1 b1) eqn:comp1.
-  - simpl in comp_eq. destruct (comp b1 c1) eqn:comp2; try discriminate.
-    + rewrite <- comp2 in comp1.
-      specialize (comp_trans a1 b1 c1 comp1) as G. rewrite <- G. rewrite comp1. rewrite comp2. reflexivity.
-    + simpl in comp_eq. specialize (comp_anti b1 c1) as G. rewrite comp2 in G. subst. rewrite comp1. reflexivity.
-  - specialize (comp_anti a1 b1) as G. rewrite comp1 in G. subst. simpl in comp_eq.
-    destruct (comp b1 c1) eqn:comp2; try assumption.
-    simpl in comp_eq.
-    specialize (comp_trans a2 b2 c2 comp_eq). apply comp_trans.
-  - simpl in comp_eq. destruct (comp b1 c1) eqn:comp2; try discriminate.
-    + simpl in comp_eq. specialize (comp_anti b1 c1) as G. rewrite comp2 in G. subst. rewrite comp1. reflexivity.
-    + rewrite <- comp2 in comp1.
-      specialize (comp_trans a1 b1 c1 comp1) as G. rewrite <- G. rewrite comp1. rewrite comp2. reflexivity.
-Qed.
-  
-Lemma bool_compare_antisymmetric : antisymmetric bool_compare.
-Proof.
-  intros a b.
-  destruct a; destruct b; reflexivity.
-Qed.
-
-Lemma bool_compare_transitive : transitive bool_compare.
-Proof.
-  intros a b c bool_compare_bc.
-  unfold bool_compare in *.
-  destruct a; destruct b; destruct c; try discriminate; reflexivity.
-Qed.
-
-Lemma b2_compare_antisymmetric : antisymmetric b2_compare.
-Proof.
-  apply if_equal_pair_antisymmetric. apply bool_compare_antisymmetric.
-Qed.
-
-Lemma b2_compare_transitive : transitive b2_compare.
-Proof.
-  apply if_equal_pair_transitive. apply bool_compare_antisymmetric. apply bool_compare_transitive.
-Qed.
-
-Lemma b4_compare_antisymmetric : antisymmetric b4_compare.
-Proof.
-  intros a b.
-  to_bits a. to_bits b.
-  unfold b4_compare, if_equal.
-  specialize (b2_compare_antisymmetric (b2, b3) (b5, b6)) as b2_comp.
-  destruct (b2_compare (b2, b3) (b5, b6)) eqn:comp1; rewrite b2_comp; auto.
-  specialize (b2_compare_antisymmetric (b1, b0) (b, b4)) as b2_comp2. inversion b2_comp. subst.
-  destruct (b2_compare (b1, b0) (b, b4)) eqn:comp2.
-  - rewrite comp1. apply b2_comp2.
-  - inversion b2_comp2. reflexivity.
-  - rewrite comp1. apply b2_comp2.
-Qed.
-
-Lemma b4_compare_transitive : transitive b4_compare.
-Proof.
-  intros a b c comp.
-  destruct a as [[[a1 a2] a3] a4]. destruct b as [[[b1 b2] b3] b4].
-  destruct c as [[[c1 c2] c3] c4].
-  unfold b4_compare in *.
-  specialize (if_equal_pair_transitive b2_compare b2_compare_antisymmetric b2_compare_transitive) as G.
-  unfold transitive in G.
-  specialize (G ((a1,a2), (a3, a4)) ((b1, b2), (b3, b4)) ((c1, c2), (c3, c4))). simpl in G. apply G in comp. apply comp.
-Qed.
-
-Lemma byte_compare_antisymmetric : antisymmetric byte_compare.
+Lemma byte_compare_antisymmetric : forall byte1 byte2, byte_compare byte1 byte2 = CompOpp (byte_compare byte2 byte1).
 Proof.
   intros byte1 byte2.
-  unfold byte_compare, if_equal; to_bits byte1; to_bits byte2.
-  specialize (b4_compare_antisymmetric (b6, b5, b4, b3) (b14, b13, b12, b11)) as G.
-  destruct (b4_compare (b6, b5, b4, b3) (b14, b13, b12, b11)) eqn:comp1; rewrite G; auto.
-  inversion G. subst.
-  specialize (b4_compare_antisymmetric (b2, b1, b0, b) (b10, b9, b8, b7)) as G1.
-  destruct (b4_compare (b2, b1, b0, b) (b10, b9, b8, b7)) eqn:comp2.
-  - rewrite antisymmetric_reflexive. assumption. apply b4_compare_antisymmetric.
-  - inversion G1. reflexivity.
-  - rewrite antisymmetric_reflexive. assumption. apply b4_compare_antisymmetric.
+  unfold byte_compare.
+  apply PeanoNat.Nat.compare_antisym.
 Qed.
 
-Lemma byte_compare_transitive : transitive byte_compare.
+Lemma byte_compare_eq_iff : forall b1 b2, byte_compare b1 b2 = Eq <-> b1 = b2.
 Proof.
-  intros a b c compare_ab_bc.
-  unfold byte_compare in *.
-  destruct (Byte.to_bits a) as [a1 [a2 [a3 [a4 [a5 [a6 [a7 a8]]]]]]].
-  destruct (Byte.to_bits b) as [b1 [b2 [b3 [b4 [b5 [b6 [b7 b8]]]]]]].
-  destruct (Byte.to_bits c) as [c1 [c2 [c3 [c4 [c5 [c6 [c7 c8]]]]]]].
-  specialize (if_equal_pair_transitive b4_compare b4_compare_antisymmetric b4_compare_transitive) as G.
-  unfold transitive in G.
-  specialize (G ((a8, a7, a6, a5), (a4,a3,a2,a1)) ((b8, b7, b6, b5), (b4,b3,b2,b1)) ((c8, c7, c6, c5), (c4,c3,c2,c1))). simpl in G. unfold b4_compare, b2_compare in compare_ab_bc. apply G in compare_ab_bc. apply compare_ab_bc.
+  intros b1 b2.
+  unfold byte_compare.
+  specialize (PeanoNat.Nat.compare_eq_iff (Byte.to_nat b1) (Byte.to_nat b2)) as [G1 G2].
+  split; intros.
+  - apply G1 in H. apply (f_equal Byte.of_nat) in H. do 2 rewrite Byte.of_to_nat in H. inversion H. reflexivity.
+  - subst. specialize (G2 ltac:(reflexivity)).
+    apply G2.
 Qed.
 
-Lemma codepoint_compare_antisymmetric : antisymmetric codepoint_compare.
-  intros a b.
-  unfold codepoint_compare, if_equal. to_bits a. to_bits b.
-  repeat
-    let comp_eq := fresh "comp_eq" in
-    let comp_spec := fresh "comp_eq" in
-    match goal with
-    | [|- context[match bool_compare ?a ?b with | _ => _ end]] =>
-        specialize (bool_compare_antisymmetric a b) as comp_spec;
-        destruct (bool_compare a b) eqn:comp_eq;
-        try rewrite comp_spec; try rewrite comp_eq
-    | [|- context[match b4_compare ?a ?b with | _ => _ end]] =>
-        specialize (b4_compare_antisymmetric a b) as comp_spec;
-        destruct (b4_compare a b) eqn:comp_eq;
-        try rewrite comp_spec; try rewrite comp_eq
-    end; try discriminate; auto.
-Qed.
-
-Lemma codepoint_compare_transitive : transitive codepoint_compare.
-  intros a b c compare_ab_bc.
-  to_bits a. to_bits b. to_bits c.
-  unfold codepoint_compare in *.
-  Admitted.
-
-Lemma lexicographic_compare_antisymmetric {T} (comp: T -> T -> comparison):
-  antisymmetric comp ->
-  antisymmetric (lexicographic_compare comp).
+Lemma list_compare_refl_if {T} (cmp: T -> T -> comparison) : forall (t: list T), 
+    (forall x y, cmp x y = Eq <-> x = y) ->
+    list_compare cmp t t = Eq.
 Proof.
-  intros comp_spec. intros a.
-  induction a as [|a a_tail]; intros b; destruct b as [|b b_tail] ; simpl; auto.
-  unfold if_equal.
-  specialize (comp_spec a b) as comp_spec1.
-  destruct (comp a b) eqn:comp1; rewrite comp_spec1; auto. subst. rewrite comp1.
-  specialize (IHa_tail b_tail).
-  destruct (lexicographic_compare comp a_tail b_tail) eqn: comp2; try assumption; subst; reflexivity.
+  intros t cmp_eq.
+  apply list_compare_refl; [| reflexivity].
+  apply cmp_eq.
 Qed.
-
-
-Lemma lexicographic_compare_transitive {T} (comp: T -> T -> comparison):
-  antisymmetric comp ->
-  transitive comp ->
-  transitive (lexicographic_compare comp).
-Proof.
-  intros comp_anti comp_trans. intro a. induction a; intros b c compare_ab_bc.
-  - destruct b; simpl in *.
-    + destruct c; tauto.
-    + destruct c; auto. discriminate.
-  - destruct b; destruct c; simpl in *; try discriminate; try tauto.
-    specialize (comp_trans a t t0).
-    specialize (comp_anti a t) as anti1.
-    specialize (comp_anti t t0) as anti2.
-    destruct (comp a t) eqn:comp1; destruct (comp t t0) eqn:comp2; simpl in *; subst; try discriminate; try tauto.
-    + specialize (comp_trans ltac:(reflexivity)). rewrite <- comp_trans. reflexivity.
-    + rewrite comp1. reflexivity.
-    + rewrite comp2. simpl. apply compare_ab_bc.
-    + rewrite antisymmetric_reflexive. simpl. apply IHa. apply compare_ab_bc. assumption.
-    + rewrite comp2. simpl. assumption.
-    + rewrite comp1. simpl. reflexivity.
-    + specialize (comp_trans ltac:(reflexivity)). rewrite <- comp_trans. reflexivity.
-Qed.
-
-
-Lemma codepoints_compare_antisymmetric : antisymmetric codepoints_compare.
-Proof.
-  apply lexicographic_compare_antisymmetric.
-  apply codepoint_compare_antisymmetric.
-Qed.
-
-Lemma codepoints_compare_transitive : transitive codepoints_compare.
-Proof.
-  apply lexicographic_compare_transitive.
-  apply codepoint_compare_antisymmetric.
-  apply codepoint_compare_transitive.
-Qed.
-
-Lemma bytes_compare_antisymmetric : antisymmetric bytes_compare.
-Proof.
-  apply lexicographic_compare_antisymmetric.
-  apply byte_compare_antisymmetric.
-Qed.
-
-
-Lemma bytes_compare_transitive : transitive bytes_compare.
-Proof.
-  apply lexicographic_compare_transitive.
-  apply byte_compare_antisymmetric.
-  apply byte_compare_transitive.
-Qed.
-
-Lemma lexicographic_compare_nil_smallest {T} (comp: T -> T -> comparison):
-  forall ts,
-    antisymmetric comp ->
-    lexicographic_compare comp nil ts = More -> False.
-Proof.
-  intros ts comp_anti compare_nil.
-  destruct ts; discriminate.
-Qed.  
