theories/Theorems/Spec.v
@@ -1,466 +1,45 @@
 From Coq Require Import Strings.Byte.
 From Coq Require Import Lia.
+From Coq Require Import Lists.List. Import ListNotations.
+From Coq Require Import ZArith.BinInt.
 
 Require Import Utf8.Parser.
 Require Import Utf8.Spec.
 Require Import Utf8.Theorems.Order.
 
-Local Notation "1" := true.
-Local Notation "0" := false.
-
-Lemma byte_range_of_bits_00_7f: forall b1 b2 b3 b4 b5 b6 b7,
-    byte_range (of_bits (b1, (b2, (b3, (b4, (b5, (b6, (b7, 0)))))))) = Range_00_7F.
-Proof.
-  intros.
-  simpl. unfold byte_range.
-  
-  destruct (of_bits (b1, (b2, (b3, (b4, (b5, (b6, (b7, 0)))))))) eqn:H;
-    apply (f_equal Byte.to_bits) in H;
-    rewrite Byte.to_bits_of_bits in H;
-    inversion H;
-    reflexivity.
-Qed.
-
-Lemma byte_range_of_bits_c2_df: forall b1 b2 b3 b4 b5,
-    (b2 = 1 \/ b3 = 1 \/ b4 = 1 \/ b5 = 1) ->
-    byte_range (of_bits (b1, (b2, (b3, (b4, (b5, (0, (1, 1)))))))) = Range_C2_DF.
-Proof.
-  intros.
-  destruct (of_bits (b1, (b2, (b3, (b4, (b5, (0, (1, 1)))))))) eqn:H2;
-    apply (f_equal Byte.to_bits) in H2;
-    rewrite Byte.to_bits_of_bits in H2;
-    inversion H2;
-    try reflexivity; destruct H as [G | [G | [G | G]]]; subst;
-    match goal with
-    | [F: 1 = 0 |- _] => apply Bool.diff_true_false in F; destruct F
-    end.
-Qed.
-
-Lemma byte_range_of_bits_a0_bf: forall b1 b2 b3 b4 b5,
-    byte_range (of_bits (b1, (b2, (b3, (b4, (b5, (1, (0, 1)))))))) = Range_A0_BF.
-Proof.
-  intros.
-  destruct (of_bits (b1, (b2, (b3, (b4, (b5, (1, (0, 1)))))))) eqn:H;
-    apply (f_equal Byte.to_bits) in H;
-    rewrite Byte.to_bits_of_bits in H;
-    inversion H;
-    reflexivity.
-Qed.
-
-Lemma byte_range_of_bits_80_8f: forall (b1 b2 b3 b4: bool),
-    byte_range (of_bits (b1, (b2, (b3, (b4, (0, (0, (0, 1)))))))) = Range_80_8F.
-Proof.
-  intros.
-  destruct (of_bits (b1, (b2, (b3, (b4, (0, (0, (0, 1)))))))) eqn:H;
-    apply (f_equal Byte.to_bits) in H;
-    rewrite Byte.to_bits_of_bits in H;
-    inversion H;
-    auto.
-Qed.
-
-
-Lemma byte_range_of_bits_80_9f: forall (b1 b2 b3 b4 b5: bool),
-    let b := of_bits (b1, (b2, (b3, (b4, (b5, (0, (0, 1))))))) in
-    (byte_range b = Range_80_8F) \/
-      (byte_range b = Range_90_9F).
-Proof.
-  intros.
-  destruct b eqn:H;
-    apply (f_equal Byte.to_bits) in H;
-    subst b;
-    rewrite Byte.to_bits_of_bits in H;
-    inversion H;
-    auto.
-Qed.
-
-Lemma byte_range_of_bits_90_bf_p1: forall (b1 b2 b3 b4 b5: bool),
-    let b := of_bits (b1, (b2, (b3, (b4, (b5, (1, (0, 1))))))) in
-    byte_range b = Range_90_9F \/ byte_range b = Range_A0_BF.
-Proof.
-    intros.
-    destruct b eqn:H;
-      apply (f_equal Byte.to_bits) in H;
-      subst b;
-      rewrite Byte.to_bits_of_bits in H;
-      inversion H;
-      auto.
-Qed.
-
-Lemma byte_range_of_bits_80_bf: forall (b1 b2 b3 b4 b5 b6: bool),
-    let b := of_bits (b1, (b2, (b3, (b4, (b5, (b6, (0, 1))))))) in
-    (byte_range b = Range_80_8F) \/
-      (byte_range b = Range_90_9F) \/
-      (byte_range b = Range_A0_BF).
-Proof.
-  intros.
-  destruct b eqn:H;
-    apply (f_equal Byte.to_bits) in H;
-    subst b;
-    rewrite Byte.to_bits_of_bits in H;
-    inversion H;
-    auto.
-Qed.
-
-Lemma byte_range_of_bits_90_9f: forall (b1 b2 b3 b4: bool),
-    let b := of_bits (b1, (b2, (b3, (b4, (1, (0, (0, 1))))))) in
-    (byte_range b = Range_90_9F).
-Proof.
-  intros.
-  destruct b eqn:H;
-    apply (f_equal Byte.to_bits) in H;
-    subst b;
-    rewrite Byte.to_bits_of_bits in H;
-    inversion H;
-    auto.
-Qed.
-
-
-Lemma byte_range_of_bits_e0 :
-  byte_range (of_bits (0, (0, (0, (0, (0, (1, (1, 1)))))))) = Byte_E0.
-Proof.
-    destruct (of_bits (0, (0, (0, (0, (0, (1, (1, 1)))))))) eqn:B;
-    apply (f_equal Byte.to_bits) in B;
-    rewrite Byte.to_bits_of_bits in B;
-    inversion B;
-    reflexivity.
-Qed.
-
-Lemma byte_range_of_bits_e1_ec: forall b1 b2 b3 b4,
-    ((b1 = 1 \/ b2 = 1 \/ b3 = 1 \/ b4 = 1) /\ (b3 = 0 \/ b4 = 0 \/ (b1 = 0 /\ b2 = 0))) ->
-  byte_range (of_bits (b1, (b2, (b3, (b4, (0, (1, (1, 1)))))))) = Range_E1_EC.
-Proof.
-  intros b1 b2 b3 b4 [[G| [G | [G | G]]] [G2 | [G2 | [G2 G3]]]]; match goal with
-  | |- byte_range ?byte = _ => destruct byte eqn:B
-  end; apply (f_equal Byte.to_bits) in B;
-    rewrite Byte.to_bits_of_bits in B;
-    inversion B;
-    subst; easy.
-Qed.
-
-
-Lemma byte_range_of_bits_ed:
-  byte_range (of_bits (1, (0, (1, (1, (0, (1, (1, 1)))))))) = Byte_ED.
-Proof.
-  destruct (of_bits (1, (0, (1, (1, (0, (1, (1, 1)))))))) eqn:B;
-    apply (f_equal Byte.to_bits) in B;
-    rewrite Byte.to_bits_of_bits in B;
-    inversion B;
-    reflexivity.
-Qed.
-
-Lemma byte_range_of_bits_ee_ef: forall (bit: bool),
-    let b := of_bits (bit, (1, (1, (1, (0, (1, (1, 1))))))) in
-    byte_range b = Range_EE_EF.
-Proof.
-  intros.
-  destruct b eqn:H;
-    apply (f_equal Byte.to_bits) in H;
-    subst b;
-    rewrite Byte.to_bits_of_bits in H;
-    inversion H;
-    auto.
-Qed.
-
-Lemma byte_range_of_bits_f0 :
-  byte_range (of_bits (0, (0, (0, (0, (1, (1, (1, 1)))))))) = Byte_F0.
-Proof.
-  destruct (of_bits (0, (0, (0, (0, (1, (1, (1, 1)))))))) eqn:H;
-    apply (f_equal Byte.to_bits) in H;
-    rewrite Byte.to_bits_of_bits in H; inversion H; reflexivity.
-Qed.
-    
-
-Lemma byte_range_of_bits_f1_f3: forall b1 b2,
-    (b1 = 1 \/ b2 = 1) ->
-    byte_range (of_bits (b1, (b2, (0, (0, (1, (1, (1, 1)))))))) = Range_F1_F3.
-Proof.
-  intros.
-  destruct (of_bits (b1, (b2, (0, (0, (1, (1, (1, 1)))))))) eqn:G;
-    apply (f_equal Byte.to_bits) in G;
-    rewrite Byte.to_bits_of_bits in G;
-    inversion G; destruct H; subst; try discriminate;
-    auto.
-Qed.
-
-Lemma byte_range_of_bits_f4:
-    let b := of_bits (0, (0, (1, (0, (1, (1, (1, 1))))))) in
-    byte_range b = Byte_F4.
-Proof.
-  intros.
-  destruct b eqn:H;
-    apply (f_equal Byte.to_bits) in H;
-    subst b;
-    rewrite Byte.to_bits_of_bits in H;
-    inversion H;
-    auto.
-Qed.
-
-
-Lemma byte_f4_bits : forall b,
-    byte_range b = Byte_F4 ->
-    Byte.to_bits b = (0, (0, (1, (0, (1, (1, (1, 1))))))).
-Proof.
-  intros.
-  destruct b; inversion H; reflexivity.
-Qed.
-
-Lemma byte_range_00_7f_bits : forall b,
-    byte_range b = Range_00_7F ->
-    exists b1 b2 b3 b4 b5 b6 b7,
-      Byte.to_bits b = (b1, (b2, (b3, (b4, (b5, (b6, (b7, 0))))))).
-Proof.
-  intros.
-  destruct b; inversion H; repeat eexists.
-Qed.
-
-Lemma byte_range_80_8f_bits : forall b,
-    byte_range b = Range_80_8F ->
-    exists b1 b2 b3 b4,
-      Byte.to_bits b = (b1, (b2, (b3, (b4, (0, (0, (0, 1))))))).
-Proof.
-  intros.
-  destruct b; inversion H; repeat eexists.
-Qed.
-
-Lemma byte_range_90_9f_bits : forall b,
-    byte_range b = Range_90_9F ->
-    exists b1 b2 b3 b4,
-      Byte.to_bits b = (b1, (b2, (b3, (b4, (1, (0, (0, 1))))))).
-Proof.
-  intros.
-  destruct b; inversion H; repeat eexists.
-Qed.
-
-Lemma byte_range_a0_bf_bits : forall b,
-    byte_range b = Range_A0_BF ->
-    exists b1 b2 b3 b4 b5,
-      Byte.to_bits b = (b1, (b2, (b3, (b4, (b5, (1, (0, 1))))))).
-Proof.
-  intros.
-  - destruct b; inversion H; repeat eexists.
-Qed.
-
-Lemma byte_range_c0_c1_bits : forall b,
-    byte_range b = Range_C0_C1 ->
-    exists b1,
-      Byte.to_bits b = (b1, (0, (0, (0, (0, (0, (1, 1))))))).
-Proof.
-  intros.
-  destruct b; inversion H; repeat eexists.
-Qed.
-
-Lemma byte_range_c2_df_bits : forall b,
-    byte_range b = Range_C2_DF ->
-    exists b1 b2 b3 b4 b5,
-      (Byte.to_bits b = (b1, (b2, (b3, (b4, (b5, (0, (1, 1))))))) /\
-       (b2 = 1 \/ b3 = 1 \/ b4 = 1 \/ b5 = 1)).
-Proof.
-  intros.
-  destruct b; inversion H; repeat eexists; auto. 
-Qed.
-
-Lemma byte_e0_bits : forall b,
-    byte_range b = Byte_E0 ->
-    (Byte.to_bits b = (0, (0, (0, (0, (0, (1, (1, 1)))))))).
-Proof.
-  intros.
-  destruct b; inversion H; reflexivity.
-Qed.
-
-Lemma byte_range_e1_ec_bits : forall b,
-    byte_range b = Range_E1_EC ->
-    exists b1 b2 b3 b4,
-      Byte.to_bits b = (b1, (b2, (b3, (b4, (0, (1, (1, 1))))))) /\ ((b1 = 1 \/ b2 = 1 \/ b3 = 1 \/ b4 = 1) /\ (b3 = 0 \/ b4 = 0 \/ (b1 = 0 /\ b2 = 0))).
-Proof.
-  intros.
-  destruct b; inversion H; repeat eexists; auto.
-Qed.
-
-
-Lemma byte_ed_bits : forall b,
-    byte_range b = Byte_ED ->
-    (Byte.to_bits b = (1, (0, (1, (1, (0, (1, (1, 1)))))))).
-Proof.
-  intros.
-  destruct b; inversion H; reflexivity.
-Qed.
-
-
-Lemma byte_range_ee_ef_bits : forall b,
-    byte_range b = Range_EE_EF ->
-    exists bit,
-      Byte.to_bits b = (bit, (1, (1, (1, (0, (1, (1, 1))))))).
-Proof.
-  intros.
-  destruct b; inversion H; repeat eexists.
-Qed.
-
-Lemma byte_f0_bits : forall b,
-    byte_range b = Byte_F0 ->
-    Byte.to_bits b = (0, (0, (0, (0, (1, (1, (1, 1))))))).
-Proof.
-  intros.
-  destruct b; inversion H; reflexivity.
-Qed.
-
-
-Lemma byte_range_f1_f3_bits : forall b,
-    byte_range b = Range_F1_F3 ->
-    exists b1 b2,
-      Byte.to_bits b = (b1, (b2, (0, (0, (1, (1, (1, 1))))))) /\
-        (b1 = 1 \/ b2 = 1).
-Proof.
-  intros.
-  destruct b; inversion H; repeat eexists; auto.
-Qed.
-
-
-Lemma byte_range_f5_ff_bits : forall b,
-    byte_range b = Range_F5_FF ->
-    exists b1 b2 b3 b4,
-      Byte.to_bits b = (b1, (b2, (b3, (b4, (1, (1, (1, 1))))))).
-Proof.
-  intros.
-  destruct b; inversion H; repeat eexists.
-Qed.
-
-Ltac destruct_bits B :=
-  match type of B with
-  | exists (b: bool), ?P => let bit := fresh "b" in let P := fresh "byte_bits" in destruct B as [bit P]; destruct_bits P
-  | ?A /\ ?C => let p := fresh "Pred" in let b := fresh "byte_bits" in destruct B as [b p]; destruct_bits b
-  | to_bits ?b = _ => apply (f_equal Byte.of_bits) in B; rewrite Byte.of_bits_to_bits in B; rewrite B in *
-  end.
-
-
-Ltac byte_range_bits ByteRange :=
-  let new := fresh "_byte_bits" in
-  match type of ByteRange with
-  | byte_range ?byte = Range_00_7F => apply byte_range_00_7f_bits in ByteRange as new
-  | byte_range ?byte = Range_80_8F => apply byte_range_80_8f_bits in ByteRange as new
-  | byte_range ?byte = Range_90_9F => apply byte_range_90_9f_bits in ByteRange as new
-  | byte_range ?byte = Range_A0_BF => apply byte_range_a0_bf_bits in ByteRange as new
-  | byte_range ?byte = Range_C2_DF => apply byte_range_c2_df_bits in ByteRange as new
-  | byte_range ?byte = Byte_E0     => apply byte_e0_bits          in ByteRange as new
-  | byte_range ?byte = Range_E1_EC => apply byte_range_e1_ec_bits in ByteRange as new
-  | byte_range ?byte = Byte_ED     => apply byte_ed_bits          in ByteRange as new
-  | byte_range ?byte = Range_EE_EF => apply byte_range_ee_ef_bits in ByteRange as new
-  | byte_range ?byte = Byte_F0     => apply byte_f0_bits          in ByteRange as new
-  | byte_range ?byte = Range_F1_F3 => apply byte_range_f1_f3_bits in ByteRange as new
-  | byte_range ?byte = Byte_F4     => apply byte_f4_bits          in ByteRange as new
-  end; destruct_bits new.
-
-
-Ltac rewrite_bits_in_hypothesis B :=
-  unfold valid_utf8_bytes in B; fold valid_utf8_bytes in B; unfold expect in B;
-  unfold in_range_80_bf, in_range_80_8f, in_range_a0_bf, in_range_90_bf, in_range_80_9f in B;
-  match type of B with
-  | valid_utf8_bytes ?bytes =>
-      idtac
-  | True => idtac
-  | context[byte_range (of_bits (?b1, (?b2, (?b3, (?b4, (?b5, (?b6, (?b7, 0))))))))] =>
-      rewrite byte_range_of_bits_00_7f in B
-  | context[byte_range (of_bits (?b1, (?b2, (?b3, (?b4, (?b5, (0, (1, 1))))))))] =>
-      rewrite byte_range_of_bits_c2_df in B; auto
-  | context[byte_range (of_bits (?b1, (?b2, (?b3, (?b4, (?b5, (1, (0, 1))))))))] =>
-      rewrite byte_range_of_bits_a0_bf in B
-  | context[byte_range (of_bits (?b1, (?b2, (?b3, (?b4, (0, (0, (0, 1))))))))] =>
-      rewrite byte_range_of_bits_80_8f in B
-  | context[byte_range (of_bits (?b1, (?b2, (?b3, (?b4, (1, (0, (0, 1))))))))] =>
-      rewrite byte_range_of_bits_90_9f in B
-  | context[byte_range (of_bits (0, (0, (0, (0, (0, (1, (1, 1))))))))] =>
-      rewrite byte_range_of_bits_e0 in B
-  | context[byte_range (of_bits (1, (0, (1, (1, (0, (1, (1, 1))))))))] =>
-      rewrite byte_range_of_bits_ed in B
-  | context[byte_range (of_bits (?bit, (1, (1, (1, (0, (1, (1, 1))))))))] =>
-      rewrite byte_range_of_bits_ee_ef in B
-  | context[byte_range (of_bits (?b1, (?b2, (?b3, (?b4, (0, (1, (1, 1))))))))] =>
-      rewrite byte_range_of_bits_e1_ec in B; auto
-  | context[byte_range (of_bits (0, (0, (1, (0, (1, (1, (1, 1))))))))] =>
-      rewrite byte_range_of_bits_f4 in B
-  | context[byte_range (of_bits (0, (0, (0, (0, (1, (1, (1, 1))))))))] =>
-      rewrite byte_range_of_bits_f0 in B
-  | context[byte_range (of_bits (?b1, (?b2, (0, (0, (1, (1, (1, 1))))))))] =>
-      rewrite byte_range_of_bits_f1_f3 in B; auto
-  | ?a /\ ?b =>
-      let P1 := fresh "P1" in let P2 := fresh "P2" in
-                              destruct B as [P1 P2]; rewrite_bits_in_hypothesis P1; rewrite_bits_in_hypothesis P2
-  end.
-
-Ltac validate_utf8_bytes :=
-  unfold valid_utf8_bytes; fold valid_utf8_bytes; unfold expect;
-  repeat match goal with
-    | [ |- valid_utf8_bytes nil ] => unfold valid_utf8_bytes
-    | [ |- True ] => constructor
-    | [ |- ?A /\ ?B ] => split
-    | [ |- context[byte_range (of_bits (?b1, (?b2, (?b3, (?b4, (?b5, (?b6, (?b7, 0))))))))]] =>
-        rewrite byte_range_of_bits_00_7f
-    | [ |- context[byte_range (of_bits (?b1, (?b2, (?b3, (?b4, (?b5, (0, (1, 1))))))))]] =>
-        rewrite byte_range_of_bits_c2_df; auto
-    | [ |- context[byte_range (of_bits (0, (0, (0, (0, (0, (1, (1, 1))))))))]] =>
-        rewrite byte_range_of_bits_e0
-    | [ |- context[byte_range (of_bits (1, (0, (1, (1, (0, (1, (1, 1))))))))]] =>
-        rewrite byte_range_of_bits_ed
-    | [ |- context[byte_range (of_bits (?bit, (1, (1, (1, (0, (1, (1, 1))))))))]] =>
-        rewrite byte_range_of_bits_ee_ef
-    | [ |- context[byte_range (of_bits (?b1, (?b2, (?b3, (?b4, (0, (1, (1, 1))))))))]] =>
-        rewrite byte_range_of_bits_e1_ec; auto
-    | [ |- context[byte_range (of_bits (0, (0, (1, (0, (1, (1, (1, 1))))))))]] =>
-        rewrite byte_range_of_bits_f4
-    | [ |- context[byte_range (of_bits (0, (0, (0, (0, (1, (1, (1, 1))))))))]] =>
-        rewrite byte_range_of_bits_f0
-    | [ |- context[byte_range (of_bits (?b1, (?b2, (0, (0, (1, (1, (1, 1))))))))]] =>
-        rewrite byte_range_of_bits_f1_f3; auto
-    | [ |- in_range_80_8f (of_bits (?b1, (?b2, (?b3, (?b4, (0, (0, (0, 1)))))))) ] =>
-        let byte_bits := fresh "ByteBits" in
-        unfold in_range_80_8f;
-        rewrite byte_range_of_bits_80_8f; auto
-    | [ |- in_range_80_9f (of_bits (?b1, (?b2, (?b3, (?b4, (?b5, (0, (0, 1))))))))] =>
-          unfold in_range_80_9f;
-          destruct b5; [ rewrite byte_range_of_bits_90_9f | rewrite byte_range_of_bits_80_8f ] 
-    | [ |- in_range_90_bf (of_bits (?b1, (?b2, (?b3, (?b4, (?b5, (1, (0, 1)))))))) ] =>
-        let byte_bits := fresh "ByteBits" in
-        let bits := fresh "Bits" in
-        pose proof (byte_range_of_bits_90_bf_p1 b1 b2 b3 b4 b5) as bits;
-        unfold in_range_90_bf;
-        destruct bits as [byte_bits | byte_bits]; rewrite byte_bits
-    | [ |- in_range_90_bf (of_bits (?b1, (?b2, (?b3, (?b4, (1, (0, (0, 1)))))))) ] =>
-        unfold in_range_90_bf;
-        rewrite byte_range_of_bits_90_9f
-    | [ |- in_range_80_8f (of_bits (?b1, (?b2, (?b3, (?b4, (0, (0, (0, 1)))))))) ] =>
-        unfold in_range_80_8f;
-        rewrite byte_range_of_bits_80_8f
-    | [ |- in_range_a0_bf (of_bits (?b1, (?b2, (?b3, (?b4, (?b5, (1, (0, 1)))))))) ] =>
-        unfold in_range_a0_bf;
-        rewrite byte_range_of_bits_a0_bf
-    | [ |- in_range_80_bf (of_bits (?b1, (?b2, (?b3, (?b4, (?b5, (?b6, (0, 1))))))))] =>
-        let byte_bits := fresh "ByteBits" in
-        let bits := fresh "Bits" in
-        pose proof (byte_range_of_bits_80_bf b1 b2 b3 b4 b5 b6) as bits;
-        unfold in_range_80_bf;
-        destruct bits as [byte_bits | [byte_bits | byte_bits]]; rewrite byte_bits
-    end.
-
-Ltac destruct_valid_bytes R :=
+Ltac destruct_valid_bytes valid_bytes :=
+  let start R :=
+    match type of R with
+    | valid_utf8_bytes (cons ?head ?tail) => idtac
+    | valid_utf8_bytes ?bytes =>
+        let head := fresh "byte" in
+        let tail := fresh "byte_rest" in
+        let bytes := fresh "bytes_eq" in
+        destruct bytes as [|head tail] eqn:bytes
+    end;
+    unfold valid_utf8_bytes in valid_bytes;
+    fold valid_utf8_bytes in valid_bytes;
+    match type of R with
+    | context[byte_range ?byte] =>
+        let byte_in_range := fresh "byte_in_range" in
+        destruct (byte_range byte) eqn:byte_in_range; try contradiction
+    end
+  in
+let rec go R :=
+  unfold expect in R;
   match type of R with
-  | valid_utf8_bytes ?bytes =>
-      idtac
-  | context[byte_range ?byte] =>
-      let r := fresh "ByteRange" in
-      destruct (byte_range byte) eqn:r; try easy; byte_range_bits r;
-      destruct_valid_bytes R
-  | expect ?pred ?bytes_pred ?bytes =>
-      let b := fresh "byte" in
-      let bs := fresh "bytes" in
-      let pred := fresh "pred" in
-      let pred_rest := fresh "bytes_valid" in
-      destruct bytes as [| b bs]; try easy; simpl in R;
-      destruct R as [pred pred_rest];
-      unfold in_range_80_bf, in_range_80_8f, in_range_a0_bf, in_range_90_bf, in_range_80_9f in pred;
-      destruct_valid_bytes pred;
-      destruct_valid_bytes pred_rest
-  | True => idtac
-  end.
-
+  | valid_utf8_bytes ?b => idtac
+  | match ?bytes with | _ => _ end =>
+      let head := fresh "byte" in
+      let tail := fresh "byte_rest" in
+      let bytes_eq := fresh "bytes_eq" in
+      let byte_pred := fresh "byte_pred" in 
+      let rest_pred := fresh "rest_pred" in
+      destruct bytes as [| head tail] eqn:bytes_eq; try contradiction;
+      destruct R as [byte_pred rest_pred];
+      go rest_pred
+  end in
+  start valid_bytes; go valid_bytes.
 
 Theorem valid_utf8_bytes_concat_strong : forall (bytes_big bytes1 bytes2: list byte),
     (length bytes1) <= (length bytes_big) ->
@@ -509,23 +88,18 @@ Proof.
   - intros bytes1 bytes2 LessThan bytes_concat_valid bytes1_valid.
     destruct bytes1.
     + apply bytes_concat_valid.
-    + simpl in bytes1_valid. Opaque Byte.of_bits.
-      destruct_valid_bytes bytes1_valid; simpl in bytes_concat_valid; repeat rewrite_bits_in_hypothesis bytes_concat_valid; try contradiction; match goal with
-      | [G: valid_utf8_bytes (?bytes1 ++ ?bytes2) |- _ ]  => apply (IHbytes_big bytes1 bytes2); repeat assumption; simpl in LessThan |- *; try lia
-      end. 
+    + rewrite <- List.app_comm_cons in bytes_concat_valid.
+      destruct_valid_bytes bytes1_valid; destruct_valid_bytes bytes_concat_valid; try discriminate;
+      repeat match goal with
+             | [G: ((?byte1 :: ?bs1) ++ ?bs2)%list = (?byte2 :: ?bs3)%list |- _] =>
+                 inversion G; subst
+             | _ => idtac
+             end; 
+        match goal with 
+        | [G1: valid_utf8_bytes ?bytes1, G2: valid_utf8_bytes (?bytes1 ++ ?bytes2) |- valid_utf8_bytes ?bytes2] => 
+            apply (IHbytes_big bytes1 bytes2); try (simpl in *; lia); repeat assumption
+        end.
 Qed.
-
-Definition next_valid_codepoint (code: codepoint) : option codepoint :=
-  match code with
-  | (0, (0, 0, 0, 0), (1, 1, 0, 1), (0, 1, 1, 1), (1, 1, 1, 1), (1, 1, 1, 1)) =>
-      Some (0, b4_zero, (1, 1, 1, 0), b4_zero, b4_zero, b4_zero)
-  | (1, (0, 0, 0, 0), (1, 1, 1, 1), (1, 1, 1, 1), (1, 1, 1, 1), (1, 1, 1, 1)) =>
-      None
-  | (b1, (b2, b3, b4, b5), (b6, b7, b8, b9), (b10, b11, b12, b13), (b14, b15, b16, b17), (b18, b19, b20, b21)) =>
-      None
-  end.
-
-Require Import Coq.Lists.List. Import ListNotations.
 
 Lemma list_equals_self_append_implies_nil {T}: forall (list1 list2: list T),
     list1 = list1 ++ list2 ->
@@ -570,10 +144,10 @@ Proof.
   destruct G as [enc_implies_valid_utf8_bytes [valid_codepoints_iff_enc [enc_strictly_increasing enc_projects]]].
   intros codes1 codes2 bytes encoder_codes1 encoder_codes2.
   specialize (enc_strictly_increasing codes1 codes2 bytes bytes encoder_codes1 encoder_codes2) as compare_codes.
-  specialize (codepoints_compare_antisymmetric codes1 codes2) as G.
-  rewrite (@antisymmetric_reflexive (list byte) bytes_compare bytes_compare_antisymmetric) in compare_codes.
-  rewrite compare_codes in G.
-  apply G.
+  unfold bytes_compare in compare_codes.
+  rewrite list_compare_refl_if in compare_codes. 2: apply byte_compare_eq_iff.
+  unfold codepoints_compare in compare_codes. apply list_compare_refl in compare_codes. apply compare_codes.
+  apply Z.compare_eq_iff.
 Qed.
 
 Theorem encoder_spec_implies_encode_single_equals : forall encoder1 code bytes,
@@ -703,10 +277,10 @@ Proof.
   destruct G as [dec_implies_valid_utf8_bytes [valid_bytes_iff_enc dec_strictly_increasing]].
   intros bytes1 bytes2 codes decoder_bytes1 decoder_bytes2.
   specialize (dec_strictly_increasing bytes1 bytes2 codes codes decoder_bytes1 decoder_bytes2) as compare_codes.
-  specialize (bytes_compare_antisymmetric bytes1 bytes2) as G.
-  rewrite (@antisymmetric_reflexive (list codepoint) codepoints_compare codepoints_compare_antisymmetric) in compare_codes.
-  rewrite <- compare_codes in G.
-  apply G.
+  unfold codepoints_compare in compare_codes.
+  rewrite list_compare_refl_if in compare_codes. 2: apply Z.compare_eq_iff.
+  unfold bytes_compare in compare_codes. symmetry in compare_codes. rewrite list_compare_refl in compare_codes.
+  apply compare_codes. apply byte_compare_eq_iff.
 Qed.
 
 Lemma decoder_spec_nil_mapsto_nil : forall decoder,
@@ -752,10 +326,6 @@ Proof.
   specialize (dec_strictly_increasing bytes bytes2 codes2 codes3 decode_bytes decode_bytes2).
   rewrite <- enc_strictly_increasing in dec_strictly_increasing.
   symmetry in dec_strictly_increasing.
-  specialize (codepoints_compare_transitive codes_prefix codes2 codes3 dec_strictly_increasing) as codes_trans.
-  induction codes2.
-  - unfold codepoints_compare in *. simpl in *.
-    destruct codes3. 
 Qed.
 
 (*   intros encoder decoder encoder_spec_compliant decoder_spec_compliant. *)
